bump

Properties/Invariant.v
@@ -3635,20 +3635,11 @@ Section Proof_of_Accountability.
     n1 <> n2 /\ confirmed n1 w /\ confirmed n2 w /\ 
     (localState w n1).(submitted_value) <> (localState w n2).(submitted_value).
 
-  Variables (w : World) (n1 n2 : Address).
-  Hypothesis (H_w_reachable : reachable w) (Hfundamental : confirmed_different_values n1 n2 w).
-
-  Local Tactic Notation "prepare" :=
-    destruct Hfundamental as (Hnneq & (H_n1_nonbyz & Hn1valid & Hconf1)
-      & (H_n2_nonbyz & Hn2valid & Hconf2) & Hvneq); clear Hfundamental.
-  
-  (* Hypotheses 
-    (Hnneq : n1 <> n2)
-    (H_n1_nonbyz : is_byz n1 = false) (Hn1valid : valid_node n1)
-    (H_n2_nonbyz : is_byz n2 = false) (Hn2valid : valid_node n2)
-    (Hconf1 : (localState w n1).(conf))
-    (Hconf2 : (localState w n2).(conf))
-    (Hvneq : (localState w n1).(submitted_value) <> (localState w n2).(submitted_value)). *)
+  Definition confirmed_different_values' n1 n2 w : Prop :=
+    n1 <> n2 /\ confirmed n1 w /\ confirmed n2 w /\ 
+    (localState w n1).(submitted_value) = Some (value_bft n1) /\
+    (localState w n2).(submitted_value) = Some (value_bft n2) /\
+    value_bft n1 <> value_bft n2.
 
   Local Tactic Notation "get_submitted" hyp(Hinv) "as_" ident(v) ident(EE) :=
     match type of Hinv with node_invariant _ (localState ?w ?n) =>
@@ -3669,8 +3660,8 @@ Section Proof_of_Accountability.
       subst v
     end end.
 
-  Local Tactic Notation "saturate" :=
-    pose proof (reachable_inv _ H_w_reachable) as Hinv;
+  Local Tactic Notation "saturate" constr(n1) constr(n2) hyp(Hinv) :=
+    (* pose proof (reachable_inv _ H_w_reachable) as Hinv; *)
     pose proof Hinv as (Hcoh, Hnodeinv, _);
     match goal with 
     | H_n1_nonbyz : is_byz n1 = false, H_n2_nonbyz : is_byz n2 = false |- _ =>
@@ -3684,6 +3675,52 @@ Section Proof_of_Accountability.
     assert (value_bft n1 <> value_bft n2) as Hvneq' by eqsolve
     end.
 
+  Fact confirmed_different_values_strengthen n1 n2 w (Hinv : invariant w) :
+    confirmed_different_values n1 n2 w <-> confirmed_different_values' n1 n2 w.
+  Proof.
+    split.
+    - intros (Hnneq & (H_n1_nonbyz & Hn1valid & Hconf1) & (H_n2_nonbyz & Hn2valid & Hconf2) & Hvneq).
+      saturate n1 n2 Hinv.
+      now hnf.
+    - intros H.
+      hnf in H |- *.
+      intuition congruence.
+  Qed.
+
+  Fact confirmed_different_values'_is_invariant n1 n2 :
+    is_invariant_step (fun w => invariant w /\ confirmed_different_values' n1 n2 w).
+  Proof.
+    hnf.
+    intros q w w' (Hinv & (Hnneq & (H_n1_nonbyz & Hn1valid & Hconf1) & 
+      (H_n2_nonbyz & Hn2valid & Hconf2) & Hv1 & Hv2 & Hvneq)) Hstep.
+    split.
+    1: eapply inv_step; eauto.
+    hnf.
+    split; try assumption.
+    split; [ | split ].
+    1-2: hnf; do 2 (split; try assumption).
+    1-2: eapply honest_node_confirmed_is_invariant; eauto.
+    1-2: split; [ assumption | hnf; auto ].
+    split; [ | split; try assumption ].
+    all: eapply honest_node_submitted_is_invariant; eauto.
+    all: split; [ assumption | hnf; auto ].
+  Qed.
+
+  Variables (w : World) (n1 n2 : Address).
+  Hypothesis (H_w_reachable : reachable w) (Hfundamental : confirmed_different_values n1 n2 w).
+
+  Local Tactic Notation "prepare" hyp(H) :=
+    destruct H as (Hnneq & (H_n1_nonbyz & Hn1valid & Hconf1)
+      & (H_n2_nonbyz & Hn2valid & Hconf2) & Hvneq); clear H.
+
+  (* Hypotheses 
+    (Hnneq : n1 <> n2)
+    (H_n1_nonbyz : is_byz n1 = false) (Hn1valid : valid_node n1)
+    (H_n2_nonbyz : is_byz n2 = false) (Hn2valid : valid_node n2)
+    (Hconf1 : (localState w n1).(conf))
+    (Hconf2 : (localState w n2).(conf))
+    (Hvneq : (localState w n1).(submitted_value) <> (localState w n2).(submitted_value)). *)
+
   (* well, using 4 packets instead of 2 is inevitable. *)
   Definition mutual_lightcerts b1 b2 b3 b4 := Eval cbn in
     let f src dst b := (mkP src dst (LightConfirmMsg 
@@ -3692,8 +3729,9 @@ Section Proof_of_Accountability.
 
   Lemma mutual_lightcerts_sent : exists b1 b2 b3 b4, incl (mutual_lightcerts b1 b2 b3 b4) (sentMsgs w).
   Proof.
-    prepare.
-    saturate.
+    prepare Hfundamental.
+    pose proof (reachable_inv _ H_w_reachable) as Hinv.
+    saturate n1 n2 Hinv.
     apply inv_conf_lightconfmsg in Hnodeinv1, Hnodeinv2.
     rewrite E1 in Hnodeinv1.
     rewrite E2 in Hnodeinv2.
@@ -3733,14 +3771,15 @@ Section Proof_of_Accountability.
 
   Lemma eventually_mutual_lightcert_conflict_detected : mutual_lightcert_conflict_detected w0.
   Proof.
-    prepare.
+    prepare Hfundamental.
     pose proof reachable_is_invariant as Hq.
     apply is_invariant_step_trace in Hq.
     apply Hq in Htrace0; auto.
     rename Htrace0 into Htmp.
     rewrite <- Ew0 in *.
     clear Ew0 Hq l0.
-    saturate.
+    pose proof (reachable_inv _ H_w_reachable) as Hinv.
+    saturate n1 n2 Hinv.
     pose proof (reachable_inv_2 _ Htmp) as (Hinv2).
     eapply incl_Forall in Hinv2.
     2: apply Hw0.
@@ -3791,9 +3830,19 @@ Section Proof_of_Accountability.
           In (mkP n1 n (ConfirmMsg (value_bft n1, nsigs1)) b1) pkts /\
           In (mkP n2 n (ConfirmMsg (value_bft n2, nsigs2)) b2) pkts) }.
   Proof.
+  (* Proof using n1 n2 w0 H_w0_reachable Hfundamental0.
+    clear l0 Htrace0 Ew0 Hfundamental H_w_reachable. clear w. *)
     pose proof eventually_mutual_lightcert_conflict_detected as H.
-    prepare.
-    saturate.
+    pose proof (reachable_inv _ H_w_reachable) as Hinv.
+    pose proof Hfundamental as Hf2.
+    (* essentially, depending on "confirmed_different_values'_is_invariant" *)
+    rewrite (confirmed_different_values_strengthen _ _ _ Hinv) in Hf2.
+    pose proof (confirmed_different_values'_is_invariant n1 n2) as Hinv'%is_invariant_step_trace.
+    specialize (Hinv' _ _ (conj Hinv Hf2) Htrace0).
+    rewrite <- Ew0 in Hinv'.
+    destruct Hinv' as (Htmp & (Hnneq & (H_n1_nonbyz & Hn1valid & Hconf1) & 
+      (H_n2_nonbyz & Hn2valid & Hconf2) & Hv1 & Hv2 & Hvneq)).
+
     exists (filter (fun p => if good_packet_dec p 
       then (match msg p with ConfirmMsg _ => true | _ => false end) else false) 
       (sentMsgs w0)).
@@ -3802,35 +3851,13 @@ Section Proof_of_Accountability.
     split.
     1: rewrite Forall_forall; setoid_rewrite filter_In.
     1: intros p (? & ?); destruct (good_packet_dec p); eqsolve.
-    (* again, need some pure invariants here *)
     intros n Hnvalid H_n_nonbyz.
-    pose proof (honest_node_submitted_is_invariant n1 (value_bft n1)) as Hisinv1%is_invariant_step_trace.
-    pose proof (honest_node_submitted_is_invariant n2 (value_bft n2)) as Hisinv2%is_invariant_step_trace.
-    pose proof Htrace0 as E1_%Hisinv1.
-    2: split; [ | hnf ]; auto.
-    pose proof Htrace0 as E2_%Hisinv2.
-    2: split; [ | hnf ]; auto.
-    pose proof (honest_node_confirmed_is_invariant n1) as Hisinv1'%is_invariant_step_trace.
-    pose proof (honest_node_confirmed_is_invariant n2) as Hisinv2'%is_invariant_step_trace.
-    pose proof Htrace0 as E1_'%Hisinv1'.
-    2: split; [ | hnf ]; auto.
-    pose proof Htrace0 as E2_'%Hisinv2'.
-    2: split; [ | hnf ]; auto.
-    rewrite <- Ew0 in E1_, E2_, E1_', E2_'.
-    pose proof (proj1 E1_) as Htmp.
-    apply proj2 in E1_, E2_, E1_', E2_'.
-    specialize (E1_ Hn1valid H_n1_nonbyz).
-    specialize (E2_ Hn2valid H_n2_nonbyz).
-    specialize (E1_' Hn1valid H_n1_nonbyz).
-    specialize (E2_' Hn2valid H_n2_nonbyz).
-
-    (* at least we should know conf at w', to make sure full certs can be broadcast  *)
     pose proof Htmp as (Hcoh_, Hnodeinv_, _).
     pose proof (Hnodeinv_ _ H_n1_nonbyz) as Hnodeinv1_.
     pose proof (Hnodeinv_ _ H_n2_nonbyz) as Hnodeinv2_.
     apply inv_conf_confmsg in Hnodeinv1_, Hnodeinv2_.
-    rewrite E1_, E1_', (id_coh _ Hcoh_) in Hnodeinv1_.
-    rewrite E2_, E2_', (id_coh _ Hcoh_) in Hnodeinv2_.
+    rewrite Hconf1, Hv1, (id_coh _ Hcoh_) in Hnodeinv1_.
+    rewrite Hconf2, Hv2, (id_coh _ Hcoh_) in Hnodeinv2_.
     specialize (Hnodeinv1_ eq_refl (proj1 H) n Hnvalid).
     specialize (Hnodeinv2_ eq_refl (proj2 H) n Hnvalid).
     destruct Hnodeinv1_ as (b1 & Hin1), Hnodeinv2_ as (b2 & Hin2).
@@ -3857,7 +3884,6 @@ Section Proof_of_Accountability.
   Fact fullcerts_all_received_suffcond w' (H2 : incl (map receive_pkt (projT1 fullcerts_all_sent)) (sentMsgs w'))
     (Hinv : invariant w') : fullcerts_all_received w'.
   Proof.
-    
     destruct fullcerts_all_sent as (pkts & HH).
     simpl in H2.
     destruct HH as (Hincl & Hgood & Haa).
@@ -3872,7 +3898,7 @@ Section Proof_of_Accountability.
     pose proof (Hpsentinv0 _ Hin1) as Ht1.
     pose proof (Hpsentinv0 _ Hin2) as Ht2.
     simpl in Ht1, Ht2.
-    prepare.
+    prepare Hfundamental.
     rewrite H_n1_nonbyz in Ht1.
     rewrite H_n2_nonbyz in Ht2.
     eqsolve.
@@ -3937,8 +3963,9 @@ Section Proof_of_Accountability.
     clear Ew1 Hq l1.
     clear dependent w0.
     clear dependent l0.
-    prepare.
-    saturate.
+    prepare Hfundamental.
+    pose proof (reachable_inv _ H_w_reachable) as Hinv.
+    saturate n1 n2 Hinv.
     clear Hconf1 Hconf2 H_w_reachable E1 E2 Hinv Hcoh Hnodeinv Hnodeinv1 Hnodeinv2. (* TODO why clear dependent w does not work here? *)
     clear Hvneq.
     pose proof (reachable_inv _ Htmp) as Hinv.
